Iris/Iris/BI.lean
@@ -4,7 +4,6 @@ public import Iris.BI.Classes
 public import Iris.BI.DerivedLaws
 public import Iris.BI.DerivedLawsLater
 public import Iris.BI.Extensions
-public import Iris.BI.Telescopes
 public import Iris.BI.Instances
 public import Iris.BI.BI
 public import Iris.BI.Notation
