Iris/Iris/Tests.lean
@@ -3,7 +3,6 @@ module
 public import Iris.Tests.Instances
 public import Iris.Tests.InstancesImport
 public import Iris.Tests.Notation
-public import Iris.Tests.Telescopes
 public import Iris.Tests.Tactics
 public import Iris.Tests.HeapLang
 public import Iris.Tests.Language
